Full Coq 8.20.1 compatibility with no warnings.

src/Theory/Equivs/MonadJoin.v
@@ -29,12 +29,13 @@ Coercion is_applicative : Monad >-> Applicative.
 #[global] Hint Rewrite <- @join_ap : MonadJoin.
 
 Definition bind
-  {M : Type -> Type} {inst : Monad M} {A B : Type}
-  (ma : M A) (f : A -> M B) : M B := (fmap f .> join) ma.
+  {M : Type -> Type} {inst : Monad M}
+  {A B : Type} (ma : M A) (f : A -> M B) : M B :=
+    (fmap f .> join) ma.
 
 Definition compM
-  {A B C : Type} {M : Type -> Type} {inst : Monad M}
-  (f : A -> M B) (g : B -> M C) : A -> M C :=
+  {M : Type -> Type} {inst : Monad M}
+  {A B C : Type} (f : A -> M B) (g : B -> M C) : A -> M C :=
     f .> fmap g .> join.
 
 #[global] Hint Unfold bind compM compose : MonadJoin.
@@ -45,13 +46,16 @@ Notation "mx >>= f" := (bind mx f) (at level 40).
 
 End MonadNotations.
 
-Export MonadNotations.
+Import MonadNotations.
 
 Ltac mjoin :=
-  repeat (intros;
+  repeat
+  (
+    intros;
     autounfold with MonadJoin CoqMTL;
     autorewrite with MonadJoin CoqMTL;
-    f_equal; exts; try reflexivity).
+    f_equal; exts; try reflexivity
+  ).
 
 Lemma assoc :
   forall
@@ -62,6 +66,7 @@ Proof.
   unfold bind, compose; intros.
   rewrite <- !join_fmap_fmap.
   change (fun x : A => join (fmap g (f x))) with (f .> fmap g .> join).
-  rewrite !fmap_comp. unfold compose. rewrite join_fmap_join.
-  reflexivity.
+  rewrite !fmap_comp.
+  unfold compose.
+  now rewrite join_fmap_join.
 Qed.
