src/Theory/Equivs/MonadEquiv.v
@@ -1,29 +1,33 @@
 From CoqMTL Require Import Control.
 
-(** This module contains proofs that various definitions of monads are
-    equivalent. More precisely, we prove that these definitions are
-    equivalent in the sense of the ability to construct  an instance of
-    each of them from the other:
-    - the main definition used throughout the library (from Control.Monad),
-      which says that a monad is an [Applicative] functor with [bind],
-      satisfying the laws [bind_pure_l], [bind_pure_r], [bind_assoc] and
-      [bind_ap], which relates the [Applicative] and [Monad] structure
+(**
+  This module contains proofs that various definitions of monads are
+  equivalent. More precisely, we prove that these definitions are
+  equivalent in the sense of the ability to construct  an instance of
+  each of them from the other:
+  - the main definition used throughout the library (from Control.Monad),
+    which says that a monad is an [Applicative] functor with [bind],
+    satisfying the laws [bind_pure_l], [bind_pure_r], [bind_assoc] and
+    [bind_ap], which relates the [Applicative] and [Monad] structure
 
-    - the join-based definition (from Theory.Equivs.MonadJoin), which says
-      that a monad is an [Applicative] functor with [join] that satisfies
-      the laws [join_fmap_join], [join_pure], [join_fmap_pure],
-      [join_fmap_fmap] and [join_ap]
-    - the Kleisli Triple definition, which is very similar to that of
-      Theory.Equivs.MonadBind, but has different operation names and
-      some arguments flipped
+  - the join-based definition (from Theory.Equivs.MonadJoin), which says
+    that a monad is an [Applicative] functor with [join] that satisfies
+    the laws [join_fmap_join], [join_pure], [join_fmap_pure],
+    [join_fmap_fmap] and [join_ap]
+  - the Kleisli Triple definition, which is very similar to that of
+    Theory.Equivs.MonadBind, but has different operation names and
+    some arguments flipped
 
-    As of now, I can't prove that these are equivalent to the compM-based
-    definition (from Theory.Equivs.MonadComp), which says that a monad is
-    something that has monadic composition which is associative and has
-    a neutral element. *)
+  As of now, I can't prove that these are equivalent to the compM-based
+  definition (from Theory.Equivs.MonadComp), which says that a monad is
+  something that has monadic composition which is associative and has
+  a neutral element.
+*)
 
-(** First we require all the necessary modules and repack them so as to
-    refer to them by nonconflicting names. *)
+(**
+  First we require all the necessary modules and repack them so as to
+  refer to them by nonconflicting names.
+*)
 
 From CoqMTL Require MonadJoin.
 From CoqMTL Require MonadBind.
@@ -41,63 +45,69 @@ Module Comp.
 Include MonadComp.
 End Comp.
 
-(** Each proof consists of two instances, one deriving [Monad] from the
-    definition at hand and the other one deriving an instance for that
-    definition from [Monad]. *)
+(**
+  Each proof consists of two instances, one deriving [Monad] from the
+  definition at hand and the other one deriving an instance for that
+  definition from [Monad].
+*)
 
 (** * join-based definition *)
 
 #[refine]
 #[export]
-Instance Join_to_Monad
-  (M : Type -> Type) (inst : Join.Monad M) : Monad M :=
+Instance Join_to_Monad (M : Type -> Type) (inst : Join.Monad M) : Monad M :=
 {
   is_applicative := @Join.is_applicative M inst;
   bind := @Join.bind M inst
 }.
 Proof.
-  1, 2, 4: MonadJoin.mjoin.
-  apply Join.assoc.
+  - now MonadJoin.mjoin.
+  - now MonadJoin.mjoin.
+  - now apply Join.assoc.
+  - now MonadJoin.mjoin.
 Defined.
 
 #[refine]
 #[export]
-Instance Monad_to_Join (M : Type -> Type) (inst : Monad M)
-  : Join.Monad M :=
+Instance Monad_to_Join (M : Type -> Type) (inst : Monad M) : Join.Monad M :=
 {
   is_applicative := @is_applicative M inst;
   join := @join M inst
 }.
 Proof.
   all: intros; unfold join, compose; try ext x.
-  - rewrite bind_assoc, bind_fmap. unfold compose, id. reflexivity.
-  - rewrite bind_pure_l. reflexivity.
-  - rewrite bind_fmap, <- bind_pure_r. f_equal.
-  - rewrite bind_fmap, fmap_bind. f_equal.
-  - rewrite !bind_ap. monad.
+  - rewrite bind_assoc, bind_fmap.
+    now unfold compose, id.
+  - now rewrite bind_pure_l.
+  - now rewrite bind_fmap, <- bind_pure_r.
+  - now rewrite bind_fmap, fmap_bind.
+  - rewrite !bind_ap.
+    now monad.
 Defined.
 
 (** * bind-based definition *)
 
 #[refine]
 #[export]
-Instance MonadBind_to_Monad
-  (M : Type -> Type) (inst : Bind.Monad M) : Monad M :=
+Instance MonadBind_to_Monad (M : Type -> Type) (inst : Bind.Monad M) : Monad M :=
 {
   is_applicative := @MonadBind.Applicative_MonadBind M inst;
   bind := @MonadBind.bind M inst;
 }.
-Proof. all: MonadBind.mbind. Defined.
+Proof.
+  all: now MonadBind.mbind.
+Defined.
 
 #[refine]
 #[export]
-Instance Monad_to_MonadBind
-  (M : Type -> Type) (inst : Monad M) : MonadBind.Monad M :=
+Instance Monad_to_MonadBind (M : Type -> Type) (inst : Monad M) : MonadBind.Monad M :=
 {
   pure := @pure M inst;
   bind := @bind M inst;
 }.
-Proof. all: monad. Defined.
+Proof.
+  all: now monad.
+Defined.
 
 (** * Kleisli triple *)
 
@@ -105,36 +115,37 @@ From CoqMTL Require Import KleisliTriple.
 
 #[refine]
 #[export]
-Instance Monad_to_KleisliTriple
-  (M : Type -> Type) (inst : Monad M) : KleisliTriple M :=
+Instance Monad_to_KleisliTriple (M : Type -> Type) (inst : Monad M) : KleisliTriple M :=
 {
   eta := @pure M inst;
   star := fun A B => flip (@bind M inst A B);
 }.
 Proof.
-  all: unfold flip; monad.
+  all: now unfold flip; monad.
 Defined.
 
 #[refine]
 #[export]
-Instance KleisliTriple_to_Monad
-  (M : Type -> Type) (inst : KleisliTriple M) : Monad M :=
+Instance KleisliTriple_to_Monad (M : Type -> Type) (inst : KleisliTriple M) : Monad M :=
 {
   is_applicative := Applicative_Kleisli M inst;
   bind := @bind_Kleisli M inst;
 }.
-Proof. all: kleisli. Defined.
+Proof.
+  all: now kleisli.
+Defined.
 
 (** * compM-based definition *)
 
 #[refine]
 #[export]
-Instance Monad_to_MonadComp
-  (M : Type -> Type) (inst : Monad M) : MonadComp.Monad M :=
+Instance Monad_to_MonadComp (M : Type -> Type) (inst : Monad M) : MonadComp.Monad M :=
 {
   is_applicative := is_applicative;
   compM := @compM M inst;
 }.
-Proof. all: unfold compM; monad. Defined.
+Proof.
+  all: now unfold compM; monad.
+Defined.
 
 (** TODO: MonadComp_to_Monad *)
